Minor updates, example computations

src/Extraction_Cvm_Cake.v
@@ -40,6 +40,102 @@ Extract Constant hsh_params => "( undefined () )".
 (* Extract Constant + => "add". *)
 (* Extract Constant Nat.add => "(+)". *)
 
+Definition P0 : Plc. Admitted.
+Definition P1 : Plc. Admitted.
+Definition P2 : Plc. Admitted. 
+Definition attest1 : ASP_ID. Admitted.
+Definition attest2 : ASP_ID. Admitted.
+Definition appraise : ASP_ID. Admitted.
+Definition certificate : ASP_ID. Admitted.
+Definition sys : TARG_ID. Admitted.
+Require Import Manifest_Admits.
+Definition BASE_ADDR : ASP_Address. Admitted.
+
+Definition example_phrase : Term := 
+  <{
+    @ P1 [
+      (<< attest1 P1 sys >> +<+ << attest2 P1 sys >>) -> 
+      @ P2 [
+        << appraise P1 sys >> ->
+        << certificate P1 sys >>
+      ]
+    ]
+  }>.
+
+Require Import Maps StringT ErrorStMonad_Coq.
+Definition ERR_STR : StringT. Admitted.
+
+Definition AM_LIB : AM_Library := {|
+  ASPServer_Cb        := fun addr => fun _ => fun _ => fun _ => fun _ => errC (messageLift ERR_STR) ;
+  PubKeyServer_Cb     := fun addr => fun _ => errC (Runtime ERR_STR) ;
+  PlcServer_Cb        := fun addr => fun _ => errC (Runtime ERR_STR) ;
+  UUIDServer_Cb       := fun addr => fun _ => errC (Runtime ERR_STR) ;
+
+  (* Server Addresses *)
+  ASPServer_Addr    := BASE_ADDR ; 
+  PubKeyServer_Addr := BASE_ADDR ; 
+  PlcServer_Addr    := BASE_ADDR ;
+  UUIDServer_Addr   := BASE_ADDR ;
+
+  (* Local Mappings *)
+  Local_ASPS        := [
+      (attest1, (fun _ => fun _ => fun _ => fun _ => resultC passed_bs)) ;
+      (attest2, (fun _ => fun _ => fun _ => fun _ => resultC passed_bs)) ;
+      (appraise, (fun _ => fun _ => fun _ => fun _ => resultC passed_bs)) ;
+      (certificate, (fun _ => fun _ => fun _ => fun _ => resultC passed_bs))
+    ];
+  Local_Appraisal_ASPS := [];
+
+  Local_Plcs        := [];
+  Local_PubKeys     := [];
+|}.
+
+Example compute_man_gens : 
+  exists m, map_get (manifest_generator example_phrase P0) P2 = Some m ->
+  exists ac,
+    manifest_compiler m AM_LIB = ac.
+Proof.
+  assert (EqClass.eqb P0 P0 = true) by admit;
+  assert (EqClass.eqb P0 P1 = false) by admit;
+  assert (EqClass.eqb P0 P2 = false) by admit;
+  assert (EqClass.eqb P1 P0 = false) by admit;
+  assert (EqClass.eqb P1 P1 = true) by admit;
+  assert (EqClass.eqb P1 P2 = false) by admit;
+  assert (EqClass.eqb P2 P0 = false) by admit;
+  assert (EqClass.eqb P2 P1 = false) by admit;
+  assert (EqClass.eqb P2 P2 = true) by admit.
+  unfold example_phrase, manifest_generator, manifest_generator',
+    asp_manifest_generator, at_manifest_generator, manifest_update_env, 
+    asp_manifest_update, aspid_manifest_update, update_manifest_policy_targ,
+    knowsof_manifest_update.
+  simpl in *.
+  repeat (
+    try rewrite H in *;
+    try rewrite H0 in *;
+    try rewrite H1 in *;
+    try rewrite H2 in *;
+    try rewrite H3 in *;
+    try rewrite H4 in *;
+    try rewrite H5 in *;
+    try rewrite H6 in *;
+    try rewrite H7 in *;
+    simpl in *).
+  assert (EqClass.eqb certificate appraise = false). admit.
+  repeat rewrite H8 in *.
+  assert (EqClass.eqb attest2 attest1 = false). admit.
+  repeat rewrite H9 in *.
+  eexists; intros HM; inversion HM.
+  clear HM H11.
+  repeat unfold manifest_compiler, generate_Plc_dispatcher, generate_PubKey_dispatcher, 
+    generate_UUID_dispatcher, generate_ASP_dispatcher, generate_appraisal_ASP_dispatcher,
+    generate_appraisal_ASP_dispatcher', generate_ASP_dispatcher'.
+  simpl in *.
+  unfold in_dec_set.
+
+  simpl in *.
+  destruct eqb.
+
+
 
 (*
 Extract Constant get_ev => "bind get (fn st => ret (st_ev st)) : cvm_st -> coq_EvC".
